attempt to adjust induction rule for tranfer prover, failed

example/Bellman_Ford.thy
@@ -19,7 +19,7 @@ fun bf :: "nat\<times>nat \<Rightarrow> int" where
     fold
       min
       (map
-        (\<lambda>i. plus (bf (k, i)) (W i j))
+        (\<lambda>i. plus (id (\<lambda>i'. bf (k, i')) i) (W i j))
         (upt 0 n))
       (bf (k, j))"
 thm bf.simps
@@ -31,19 +31,68 @@ fun bf\<^sub>T :: "nat\<times>nat \<Rightarrow>\<^sub>T int" where
     \<langle>fold\<^sub>T\<rangle>
     . \<langle>min\<^sub>T\<rangle>
     . (\<langle>map\<^sub>T\<rangle>
-      . \<langle>\<lambda>i. \<langle>plus\<^sub>T\<rangle> . (bf\<^sub>T (k, i)) . \<langle>W i j\<rangle>\<rangle>
+      . \<langle>\<lambda>i. \<langle>plus\<^sub>T\<rangle> . (id (\<lambda>i'. bf\<^sub>T (k, i')) i) . \<langle>W i j\<rangle>\<rangle>
       . (\<langle>upt\<^sub>T\<rangle> . \<langle>0\<rangle> . \<langle>n\<rangle>))
     . (bf\<^sub>T (k, j))"
+
 term 0 (**)
+thm bf\<^sub>T.induct
   
 interpretation bf: dp_consistency bf .
+
 context
   includes lifting_syntax
 begin
+
+lemma bf_induct:
+  "\<lbrakk>\<And>j. P (0, j);
+    \<And>k j. \<lbrakk>\<And>(x::nat) i. P (k, i);
+            P (k, j)
+           \<rbrakk> \<Longrightarrow> P (Suc k, j)
+    \<rbrakk> \<Longrightarrow> P (x::nat\<times>nat)"
+  by (fact bf\<^sub>T.induct)
+
+lemma bf_inductS:
+  "\<lbrakk>\<And>j. bf.consistentS op = (bf (0, j)) (bf\<^sub>T (0, j));
+    \<And>k j. \<lbrakk>(op = ===> bf.consistentS op =) (\<lambda>i. bf (k, i)) (\<lambda>i. bf\<^sub>T (k, i));
+            bf.consistentS op = (bf (k, j)) (bf\<^sub>T (k, j))
+           \<rbrakk> \<Longrightarrow> bf.consistentS op = (bf (Suc k, j)) (bf\<^sub>T (Suc k, j))
+    \<rbrakk> \<Longrightarrow> bf.consistentS op = (bf (x::nat\<times>nat)) (bf\<^sub>T x)"
+  unfolding rel_fun_def by (metis bf_induct[of "\<lambda>x. bf.consistentS op = (bf x) (bf\<^sub>T x)"])
+  
+term 0 (**)
 lemma "bf.consistentDP bf\<^sub>T"
-  apply (rule bf.consistentDP_intro, induct_tac rule: bf\<^sub>T.induct, unfold bf\<^sub>T.simps; rule bf.consistentS_checkmem, unfold bf.simps)
+proof ((rule bf.consistentDP_intro, induct_tac rule: bf_inductS, unfold bf\<^sub>T.simps; rule bf.consistentS_checkmem, unfold bf.simps), goal_cases)
+  case [transfer_rule]: 1 show ?case by transfer_prover
+next
+  case prems[transfer_rule]: (2 _ k j)
+    show ?case
+      apply transfer_prover_start
+                          apply transfer_step
+      apply transfer_step
+                          apply transfer_step
+      apply transfer_step
+      apply transfer_step
+                          apply transfer_step
+      apply transfer_step
+                          apply transfer_step
+                          apply transfer_step
+      apply transfer_step
+                          apply transfer_step
+                          apply transfer_step
+                          apply transfer_step
+                         apply transfer_step
+                        apply transfer_step
+                       apply transfer_step
+                      apply transfer_step
+                     apply transfer_step
+        apply transfer_step
+    term 0 (**
   subgoal premises [transfer_rule] by transfer_prover
   subgoal premises prems[transfer_rule]
+    apply transfer
+      
+    thm prems
     apply transfer_prover_start
                         apply transfer_step
                         apply transfer_step
@@ -53,11 +102,13 @@ lemma "bf.consistentDP bf\<^sub>T"
                         apply transfer_step
                         apply transfer_step
                         apply transfer_step
-                        apply transfer_step
-                        apply transfer_step
-                        apply transfer_step
-                        apply transfer_step
+      
+                        
+      
       (* going wrong here *)
       (* bf\<^sub>T (Pair k i) should be proved directly by prems(1) rather than be separated *)
+    thm prems
     oops
+    thm bf.induct bf\<^sub>T.induct
+      thm bf_induct[of "\<lambda>x. bf.consistentS op = (bf x) (bf\<^sub>T x)"]
 end
